x86/RelocLinking.v
@@ -8,6 +8,7 @@
 Require Import Coqlib Integers Values Maps AST.
 Require Import Asm RelocProgram.
 Require Import Linking Errors SeqTable.
+Require Import Symbtablegen.
 Import ListNotations.
 
 Local Open Scope list_scope.
@@ -64,26 +65,53 @@ Definition update_symbtype (e: symbentry) t :=
      symbentry_size  := symbentry_size e; |}.
 
 Definition link_symb (e1 e2: symbentry) : option symbentry :=
-  match link_symbtype (symbentry_type e1) (symbentry_type e2) with
-  | None => None
-  | Some t =>
-    let sz1 := symbentry_size e1 in
-    let sz2 := symbentry_size e2 in
-    let i1 := symbentry_secindex e1 in
-    let i2 := symbentry_secindex e2 in
-    match i1, i2 with
-    | secindex_undef, secindex_undef =>
-      Some (update_symbtype e1 t)
-    | _, secindex_undef => Some e1
-    | secindex_undef, _ => Some e2
-    | _, secindex_comm =>
-      if zeq sz1 sz2 then Some e1 else None
-    | secindex_comm, _ =>
-      if zeq sz1 sz2 then Some e2 else None
-    | secindex_normal _ , secindex_normal _ => None
-    end
+  let id1 := symbentry_id e1 in
+  let id2 := symbentry_id e2 in
+  match id1, id2 with
+  | Some id1, Some id2 =>
+    if peq id1 id2 then
+      let bindty := get_bind_ty id1 in
+      match link_symbtype (symbentry_type e1) (symbentry_type e2) with
+      | None => None
+      | Some t =>
+        let sz1 := symbentry_size e1 in
+        let sz2 := symbentry_size e2 in
+        let i1 := symbentry_secindex e1 in
+        let i2 := symbentry_secindex e2 in
+        match i1, i2 with
+        | secindex_undef, secindex_undef =>
+          Some {|symbentry_id := Some id1;
+                 symbentry_bind := bindty;
+                 symbentry_type := t;
+                 symbentry_value := 0;
+                 symbentry_secindex := secindex_undef;
+                 symbentry_size := 0;
+               |}
+        | _, secindex_undef => Some e1
+        | secindex_undef, _ => Some e2
+        | secindex_comm, secindex_comm =>
+          if zeq sz1 sz2 then
+            Some {|symbentry_id := Some id1;
+                   symbentry_bind := bindty;
+                   symbentry_type := t;
+                   symbentry_value := 8 ; (* 8 is a safe alignment for any data *)
+                   symbentry_secindex := secindex_comm;
+                   symbentry_size := Z.max sz1 0;
+                 |}
+          else 
+            None
+        | _, secindex_comm =>
+          if zeq sz1 sz2 then Some e1 else None
+        | secindex_comm, _ =>
+          if zeq sz1 sz2 then Some e2 else None
+        | secindex_normal _ , secindex_normal _ => None
+        end
+      end
+    else
+      None
+  | _, _ => None
   end.
-
+ 
 Section WITH_RELOC_OFFSET.
 
 (** Relocation offsets for internal symbols 
@@ -247,27 +275,111 @@ Defined.
 
 
 (** Properties *)
-Lemma link_option_symm: forall {F V} {LF: Linker F} {LV: Linker V} 
-                          (def1 def2: option (globdef F V)),
+Local Transparent Linker_def.
+Local Transparent Linker_fundef.
+Local Transparent Linker_vardef.
+Local Transparent Linker_unit.
+Local Transparent Linker_varinit.
+
+Lemma link_unit_symm: forall (i1 i2:unit) , link i1 i2 = link i2 i1.
+Proof.
+  intros. cbn. auto.
+Qed.
+
+Lemma link_fundef_symm: forall {F} (def1 def2: (AST.fundef F)),
+    link_fundef def1 def2 = link_fundef def2 def1.
+Proof.
+  intros. destruct def1, def2; auto.
+  cbn. 
+  destruct external_function_eq; destruct external_function_eq; subst; congruence.
+Qed.
+
+Lemma link_varinit_symm: forall i1 i2,
+    link_varinit i1 i2 = link_varinit i2 i1.
+Proof.
+  intros. unfold link_varinit.
+  destruct (classify_init i1), (classify_init i2); cbn; try congruence.
+  destruct zeq; destruct zeq; subst; cbn in *; try congruence.
+Qed.
+
+Lemma link_vardef_symm: 
+  forall {V} {LV: Linker V}
+    (LinkVSymm: forall (i1 i2: V), link i1 i2 = link i2 i1)
+    (v1 v2: globvar V),
+    link_vardef v1 v2 = link_vardef v2 v1.
+Proof.
+  intros. destruct v1,v2; cbn.
+  unfold link_vardef; cbn.
+  rewrite LinkVSymm.
+  destruct (link gvar_info0 gvar_info); try congruence.
+  rewrite link_varinit_symm. 
+  destruct (link_varinit gvar_init0 gvar_init); try congruence.
+  destruct gvar_readonly, gvar_readonly0, gvar_volatile, gvar_volatile0; 
+    cbn; try congruence.
+Qed.
+
+Lemma link_def_symm: forall {F V} {LV: Linker V}
+                       (LinkVSymm: forall (i1 i2: V), link i1 i2 = link i2 i1)
+                          (def1 def2: (globdef (AST.fundef F) V)),
+    link_def def1 def2 = link_def def2 def1.
+Proof.
+  intros.
+  destruct def1, def2; auto.
+  - cbn. 
+    rewrite link_fundef_symm. auto.
+  - cbn.
+    rewrite link_vardef_symm. auto. auto.
+Qed.
+
+Lemma link_option_symm: forall {F V} {LV: Linker V} 
+                          (LinkVSymm: forall (i1 i2: V), link i1 i2 = link i2 i1)
+                          (def1 def2: option (globdef (AST.fundef F) V)),
     link_option def1 def2 = link_option def2 def1.
 Proof.
-  Admitted.
+  intros.
+  unfold link_option. destruct def1, def2; auto.
+  cbn.
+  erewrite link_def_symm; eauto.
+Qed.
 
 
 Lemma link_prog_merge_symm: 
-  forall {F V} {LF: Linker F} {LV: Linker V} (a b:option (option (globdef F V))), 
+  forall {F V} {LV: Linker V} 
+    (LinkVSymm: forall (i1 i2: V), link i1 i2 = link i2 i1)
+    (a b:option (option (globdef (AST.fundef F) V))), 
     link_prog_merge a b = link_prog_merge b a.
 Proof.
   intros. unfold link_prog_merge.
   destruct a, b; auto.
-  apply link_option_symm.
+  apply link_option_symm. auto.
+Qed.
+
+
+Lemma link_symbtype_symm: forall t1 t2,
+    link_symbtype t1 t2 = link_symbtype t2 t1.
+Proof.
+  intros. destruct t1, t2; cbn; congruence.
 Qed.
 
 Lemma link_symb_symm: forall s1 s2,
     link_symb s1 s2 = link_symb s2 s1.
 Proof.
-  Admitted.
-
+  intros.
+  unfold link_symb.
+  destruct (symbentry_id s1), (symbentry_id s2); try congruence.
+  destruct peq, peq; try congruence. 
+  subst.
+  erewrite link_symbtype_symm.
+  match goal with 
+  | [ |- (match ?a with _ => _ end) = (match ?b with _ => _ end) ] =>
+    destruct a; try congruence
+  end.
+  destruct (symbentry_secindex s1), (symbentry_secindex s2); try congruence.
+  destruct zeq, zeq; try congruence.
+  destruct zeq, zeq; try congruence.
+  destruct zeq, zeq; try congruence.
+Qed.
+  
 Lemma link_symb_merge_symm: forall a b, link_symb_merge a b = link_symb_merge b a.
 Proof.
   intros. unfold link_symb_merge.
